src/MessagePool.v
@@ -1,0 +1,366 @@
+Require Import Bool List String Peano_dec.
+Require Import Common ListSupport FMap Syntax.
+
+Set Implicit Arguments.
+
+Section MessagePool.
+  Variable (MsgT: Type).
+  Context `{HasMsg MsgT}.
+
+  Definition Queue := list MsgT.
+  Definition MessagePool := list MsgT.
+
+  Definition findMP (from to chn: IdxT) (mp: MessagePool): Queue :=
+    filter (fun msg =>
+              if msgAddr_dec (mid_addr (msg_id (getMsg msg))) (buildMsgAddr from to chn)
+              then true
+              else false) mp.
+
+  Definition firstMP (from to chn: IdxT) (mp: MessagePool) :=
+    hd_error (findMP from to chn mp).
+
+  Fixpoint deqMP (from to chn: IdxT) (mp: MessagePool): MessagePool :=
+    match mp with
+    | nil => nil
+    | msg :: mp' =>
+      if msgAddr_dec (mid_addr (msg_id (getMsg msg))) (buildMsgAddr from to chn)
+      then mp'
+      else msg :: deqMP from to chn mp'
+    end.
+
+  Definition enqMP (m: MsgT) (mp: MessagePool): MessagePool := mp ++ (m :: nil).
+
+  Definition removeMP (m: MsgT) (mp: MessagePool): MessagePool :=
+    let mid := msg_id (getMsg m) in
+    deqMP (mid_from mid) (mid_to mid) (mid_chn mid) mp.
+
+  Definition FirstMP (mp: MessagePool) (m: MsgT) :=
+    let mid := msg_id (getMsg m) in
+    firstMP (mid_from mid) (mid_to mid) (mid_chn mid) mp = Some m.
+  
+  Definition EmptyMP (mp: MessagePool) := mp = nil.
+  Definition InMP (msg: MsgT) (mp: MessagePool) := In msg mp.
+
+  Definition ForallMP (P: MsgT -> Prop) (mp: MessagePool) :=
+    Forall P mp.
+
+  Definition distributeMsgs (nmsgs: list MsgT) (mp: MessagePool): MessagePool :=
+    mp ++ nmsgs.
+
+  Fixpoint removeMsgs (dmsgs: list MsgT) (mp: MessagePool): MessagePool :=
+    match dmsgs with
+    | nil => mp
+    | dmsg :: dmsgs' =>
+      removeMsgs dmsgs' (removeMP dmsg mp)
+    end.
+  
+End MessagePool.
+
+Section Facts.
+  Variable (MsgT: Type).
+  Context `{HasMsg MsgT}.
+
+  Lemma firstMP_app_or:
+    forall (msg: MsgT) from to chn mp1 mp2,
+      firstMP from to chn (mp1 ++ mp2) = Some msg ->
+      firstMP from to chn mp1 = Some msg \/
+      firstMP from to chn mp2 = Some msg.
+  Proof.
+    induction mp1; intros; auto.
+    unfold firstMP in *; simpl in *.
+    destruct (msgAddr_dec _ _).
+    - left; inv H0; reflexivity.
+    - auto.
+  Qed.
+
+  Lemma firstMP_enqMP_or:
+    forall (msg nmsg: MsgT) from to chn mp,
+      firstMP from to chn (enqMP nmsg mp) = Some msg ->
+      msg = nmsg \/ firstMP from to chn mp = Some msg.
+  Proof.
+    intros.
+    apply firstMP_app_or in H0; destruct H0; auto.
+    unfold firstMP in H0; cbn in H0.
+    destruct (msgAddr_dec _ _); [|discriminate].
+    inv H0; auto.
+  Qed.
+
+  Lemma firstMP_distributeMsgs_or:
+    forall (msg: MsgT) from to chn nmsgs mp,
+      firstMP from to chn (distributeMsgs nmsgs mp) = Some msg ->
+      firstMP from to chn mp = Some msg \/
+      firstMP from to chn nmsgs = Some msg.
+  Proof.
+    intros.
+    apply firstMP_app_or; auto.
+  Qed.
+
+  Lemma inMP_enqMP_or:
+    forall (msg: MsgT) nmsg mp,
+      InMP msg (enqMP nmsg mp) ->
+      msg = nmsg \/ InMP msg mp.
+  Proof.
+    intros.
+    apply in_app_or in H0; destruct H0; auto.
+    Common.dest_in; auto.
+  Qed.
+
+  Lemma inMP_deqMP:
+    forall (msg: MsgT) from to chn mp,
+      InMP msg (deqMP from to chn mp) ->
+      InMP msg mp.
+  Proof.
+    induction mp; simpl; intros; auto.
+    find_if_inside; auto.
+    inv H0; auto.
+  Qed.
+
+  Lemma inMP_distributeMsgs_or:
+    forall (msg: MsgT) nmsgs mp,
+      InMP msg (distributeMsgs nmsgs mp) ->
+      In msg nmsgs \/ InMP msg mp.
+  Proof.
+    intros; apply in_app_or in H0; destruct H0; auto.
+  Qed.
+
+  Lemma firstMP_InMP:
+    forall (msg: MsgT) from to chn mp,
+      firstMP from to chn mp = Some msg ->
+      InMP msg mp.
+  Proof.
+    induction mp; simpl; intros; [discriminate|].
+    unfold firstMP in H0; simpl in H0.
+    destruct (msgAddr_dec _ _).
+    - inv H0; auto.
+    - right; apply IHmp; auto.
+  Qed.
+
+  Lemma FirstMP_InMP:
+    forall (msg: MsgT) mp,
+      FirstMP mp msg ->
+      InMP msg mp.
+  Proof.
+    unfold FirstMP; intros.
+    eapply firstMP_InMP; eauto.
+  Qed.
+
+  Lemma ForallMP_InMP_SubList:
+    forall (msgs: list MsgT) mp,
+      ForallMP (fun msg => InMP msg mp) msgs ->
+      SubList msgs mp.
+  Proof.
+    induction msgs; intros; [apply SubList_nil|].
+    inv H0.
+    apply SubList_cons; auto.
+  Qed.
+
+  Lemma ForallMP_forall:
+    forall P mp,
+      ForallMP P mp <->
+      (forall msg: MsgT, InMP msg mp -> P msg).
+  Proof.
+    intros; apply Forall_forall.
+  Qed.
+
+  Lemma ForallMP_SubList:
+    forall P (mp1 mp2: MessagePool MsgT),
+      ForallMP P mp2 ->
+      SubList mp1 mp2 ->
+      ForallMP P mp1.
+  Proof.
+    intros.
+    apply ForallMP_forall; intros.
+    eapply ForallMP_forall in H0; eauto.
+    apply H1; auto.
+  Qed.
+
+  Lemma ForallMP_enqMP:
+    forall (P: MsgT -> Prop) (msg: MsgT) mp,
+      ForallMP P mp ->
+      P msg ->
+      ForallMP P (enqMP msg mp).
+  Proof.
+    intros.
+    apply Forall_app; auto.
+  Qed.
+
+  Lemma ForallMP_deqMP:
+    forall (P: MsgT -> Prop) from to chn mp,
+      ForallMP P mp ->
+      ForallMP P (deqMP from to chn mp).
+  Proof.
+    induction mp; simpl; intros; auto.
+    inv H0.
+    find_if_inside; auto.
+    constructor; auto.
+    apply IHmp; auto.
+  Qed.
+
+  Lemma ForallMP_removeMP:
+    forall (P: MsgT -> Prop) msg mp,
+      ForallMP P mp ->
+      ForallMP P (removeMP msg mp).
+  Proof.
+    induction mp; simpl; intros; auto.
+    inv H0.
+    cbn; destruct (msgAddr_dec _ _); auto.
+    constructor; auto.
+    apply ForallMP_deqMP; auto.
+  Qed.
+
+  Lemma ForallMP_distributeMsgs:
+    forall (P: MsgT -> Prop) (nmsgs: list MsgT) mp,
+      ForallMP P mp ->
+      ForallMP P nmsgs ->
+      ForallMP P (distributeMsgs nmsgs mp).
+  Proof.
+    intros.
+    apply Forall_app; auto.
+  Qed.
+
+  Lemma ForallMP_removeMsgs:
+    forall (P: MsgT -> Prop) (dmsgs: list MsgT) mp,
+      ForallMP P mp ->
+      ForallMP P (removeMsgs dmsgs mp).
+  Proof.
+    induction dmsgs; simpl; intros; auto.
+    apply IHdmsgs.
+    apply ForallMP_removeMP; auto.
+  Qed.
+
+  Lemma ForallMP_removeOnce:
+    forall (msg_dec: forall m1 m2: MsgT, {m1 = m2} + {m1 <> m2})
+           (P: MsgT -> Prop) tmsg mp,
+      ForallMP P mp ->
+      ForallMP P (removeOnce msg_dec tmsg mp).
+  Proof.
+    induction mp; simpl; intros; auto.
+    inv H0.
+    find_if_inside; auto.
+    constructor; auto.
+    apply IHmp; auto.
+  Qed.
+  
+  Lemma deqMP_SubList:
+    forall from to chn mp,
+      SubList (deqMP from to chn mp) mp.
+  Proof.
+    induction mp; simpl; intros; [apply SubList_nil|].
+    find_if_inside.
+    - right; auto.
+    - apply SubList_cons; [left; reflexivity|].
+      apply SubList_cons_right; auto.
+  Qed.
+
+  Lemma findMP_MsgAddr:
+    forall from to chn msg mp,
+      hd_error (findMP from to chn mp) = Some msg ->
+      mid_addr (msg_id (getMsg msg)) = buildMsgAddr from to chn.
+  Proof.
+    induction mp; simpl; intros; [discriminate|].
+    destruct (msgAddr_dec _ _); auto.
+    inv H0; auto.
+  Qed.
+
+  Lemma firstMP_MsgAddr:
+    forall from to chn mp msg,
+      firstMP from to chn mp = Some msg ->
+      mid_addr (msg_id (getMsg msg)) = buildMsgAddr from to chn.
+  Proof.
+    unfold firstMP; intros.
+    eapply findMP_MsgAddr; eauto.
+  Qed.
+
+  Lemma removeMP_deqMP:
+    forall msg mid mp,
+      msg_id (getMsg msg) = mid ->
+      removeMP msg mp = deqMP (mid_from mid) (mid_to mid) (mid_chn mid) mp.
+  Proof.
+    intros; subst; reflexivity.
+  Qed.
+
+  Lemma firstMP_FirstMP:
+    forall from to chn mp msg,
+      firstMP from to chn mp = Some msg ->
+      FirstMP mp msg.
+  Proof.
+    unfold FirstMP; intros.
+    pose proof (firstMP_MsgAddr _ _ _ _ H0).
+    destruct (msg_id (getMsg msg)) as [[ ]]; cbn in *.
+    inv H1; assumption.
+  Qed.
+
+End Facts.
+
+Section Map.
+  Variables (MsgT1 MsgT2: Type).
+  Context `{HasMsg MsgT1} `{HasMsg MsgT2}.
+
+  Variable (mmap: MsgT1 -> MsgT2).
+  Hypothesis (Hmmap: forall msg, getMsg (mmap msg) = getMsg msg).
+
+  Lemma mmap_findMP:
+    forall from to chn mp,
+      findMP from to chn (map mmap mp) =
+      map mmap (findMP from to chn mp).
+  Proof.
+    induction mp; simpl; intros; auto.
+    rewrite IHmp.
+    rewrite Hmmap.
+    destruct (msgAddr_dec _ _); auto.
+  Qed.
+
+  Lemma mmap_firstMP:
+    forall from to chn mp,
+      firstMP from to chn (map mmap mp) =
+      lift mmap (firstMP from to chn mp).
+  Proof.
+    unfold firstMP; intros.
+    rewrite mmap_findMP.
+    apply eq_sym, lift_hd_error.
+  Qed.
+
+  Lemma mmap_FirstMP:
+    forall mp msg,
+      FirstMP mp msg ->
+      FirstMP (map mmap mp) (mmap msg).
+  Proof.
+    unfold FirstMP; intros.
+    rewrite mmap_firstMP.
+    rewrite Hmmap.
+    rewrite H1.
+    reflexivity.
+  Qed.
+
+  Lemma mmap_deqMP:
+    forall mp from to chn,
+      map mmap (deqMP from to chn mp) =
+      deqMP from to chn (map mmap mp).
+  Proof.
+    induction mp; simpl; intros; auto.
+    rewrite Hmmap.
+    destruct (msgAddr_dec _ _); auto.
+    simpl; rewrite IHmp; auto.
+  Qed.
+  
+  Lemma mmap_removeMP:
+    forall mp msg,
+      map mmap (removeMP msg mp) =
+      removeMP (mmap msg) (map mmap mp).
+  Proof.
+    unfold removeMP; intros.
+    rewrite Hmmap.
+    apply mmap_deqMP.
+  Qed.
+
+  Lemma mmap_distributeMsgs:
+    forall mp msgs,
+      map mmap (distributeMsgs msgs mp) =
+      distributeMsgs (map mmap msgs) (map mmap mp).
+  Proof.
+    unfold distributeMsgs; intros.
+    apply map_app.
+  Qed.
+  
+End Map.
+
